Make Assert short-circuit

vyperSmallStepScript.sml
@@ -21,7 +21,6 @@ Datatype:
   eval_continuation
   = ReturnK eval_continuation
   | AssertK expr eval_continuation
-  | AssertK1 string eval_continuation
   | RaiseK eval_continuation
   | LogK identifier eval_continuation
   | PopK eval_continuation
@@ -244,7 +243,7 @@ Definition eval_stmt_cps_def:
   eval_stmt_cps cx (Return NONE) st k = AK cx (ApplyExc (ReturnException NoneV)) st k ∧
   eval_stmt_cps cx (Return (SOME e)) st k = eval_expr_cps cx e st (ReturnK k) ∧
   eval_stmt_cps cx (Raise se) st k = eval_expr_cps cx se st (RaiseK k) ∧
-  eval_stmt_cps cx (Assert e se) st k = eval_expr_cps cx se st (AssertK e k) ∧
+  eval_stmt_cps cx (Assert e se) st k = eval_expr_cps cx e st (AssertK se k) ∧
   eval_stmt_cps cx (Log id es) st k = eval_exprs_cps cx es st (LogK id k) ∧
   eval_stmt_cps cx (AnnAssign id typ e) st k =
     eval_expr_cps cx e st (AnnAssignK id k) ∧
@@ -313,7 +312,6 @@ val () = apply_def
 Definition apply_exc_def:
   apply_exc cx ex st (ReturnK k) = AK cx (ApplyExc ex) st k ∧
   apply_exc cx ex st (AssertK _ k) = AK cx (ApplyExc ex) st k ∧
-  apply_exc cx ex st (AssertK1 _ k) = AK cx (ApplyExc ex) st k ∧
   apply_exc cx ex st (RaiseK k) = AK cx (ApplyExc ex) st k ∧
   apply_exc cx ex st (LogK _ k) = AK cx (ApplyExc ex) st k ∧
   apply_exc cx ex st (AppendK _ k) = AK cx (ApplyExc ex) st k ∧
@@ -475,18 +473,13 @@ val () = apply_tv_def
 
 Definition apply_val_def:
   apply_val cx v st (ReturnK k) = apply_exc cx (ReturnException v) st k ∧
-  apply_val cx (BoolV T) st (AssertK1 str k) = apply cx st k ∧
-  apply_val cx (BoolV F) st (AssertK1 str k) =
-    apply_exc cx (AssertException str) st k ∧
-  apply_val cx v st (AssertK1 _ k) = apply_exc cx (Error "not BoolV") st k ∧
-  apply_val cx (StringV _ str) st (AssertK e k) =
-    eval_expr_cps cx e st (AssertK1 str k) ∧
+  apply_val cx (BoolV T) st (AssertK se k) = apply cx st k ∧
+  apply_val cx (BoolV F) st (AssertK se k) = eval_expr_cps cx se st (RaiseK k) ∧
+  apply_val cx _ st (AssertK e k) = apply_exc cx (Error "not BoolV") st k ∧
   apply_val cx (StringV _ str) st (RaiseK k) =
     apply_exc cx (AssertException str) st k ∧
   apply_val cx _ st (RaiseK k) =
-    apply_exc cx (Error "raise not StringV") st k ∧
-  apply_val cx _ st (AssertK e k) =
-    apply_exc cx (Error "assert not StringV") st k ∧
+    apply_exc cx (Error "not StringV") st k ∧
   apply_val cx v st (AnnAssignK id k) =
     liftk cx (K Apply) (new_variable id v st) k ∧
   apply_val cx v st (AssignK1 gv k) =
@@ -731,40 +724,53 @@ Proof
     \\ CASE_TAC \\ rw[cont_def] \\ reverse CASE_TAC
     >- rw[Once OWHILE_THM, stepk_def, apply_exc_def]
     \\ rw[Once OWHILE_THM, stepk_def, apply_tv_def, liftk1]
-    \\ CASE_TAC
-    \\ CASE_TAC \\ rw[Once OWHILE_THM, stepk_def, apply_exc_def]
-    \\ qmatch_goalsub_rename_tac`dest_StringV v`
-    \\ first_x_assum $ drule_then drule
-    \\ rw[cont_def]
-    \\ CASE_TAC \\ CASE_TAC \\ gvs[]
-    \\ BasicProvers.TOP_CASE_TAC \\ gvs[]
-    \\ pop_assum mp_tac
-    \\ reverse BasicProvers.TOP_CASE_TAC \\ gvs[]
-    \\ strip_tac \\ gvs[]
-    >- (
-      Cases_on`v` \\ gvs[dest_StringV_def, lift_option_def, raise_def,
-                         apply_val_def, return_def]
-      \\ rw[Once OWHILE_THM, SimpRHS, stepk_def, apply_exc_def] \\ gvs[]
-      \\ rw[apply_exc_def] \\ rw[Once OWHILE_THM] )
-    \\ Cases_on`v` \\ gvs[dest_StringV_def, lift_option_def, raise_def,
-                       apply_val_def, return_def]
-    \\ pop_assum mp_tac
-    \\ reverse CASE_TAC \\ strip_tac \\ gvs[]
-    >- rw[Once OWHILE_THM, stepk_def, apply_exc_def]
-    \\ rw[Once OWHILE_THM, stepk_def] \\ gvs[apply_tv_def, liftk1, return_def]
     \\ qmatch_goalsub_rename_tac`get_Value v`
-    \\ Cases_on`v` \\ gvs[return_def, raise_def]
-    \\ rw[Once OWHILE_THM, stepk_def, apply_val_def, apply_exc_def]
-    \\ gvs[switch_BoolV_def, raise_def]
-    \\ pop_assum mp_tac
-    \\ reverse(rw[return_def, raise_def]) \\ rw[apply_val_def]
+    \\ reverse $ Cases_on`v` \\ rw[return_def, raise_def]
     >- (
-      qmatch_goalsub_rename_tac`apply_val _ v`
-      \\ Cases_on`v` \\ rw[apply_val_def]
-      \\ rw[Once OWHILE_THM, stepk_def, SimpRHS] \\ gvs[]
-      \\ rw[apply_exc_def, Once OWHILE_THM] )
-    \\ rw[Once OWHILE_THM, stepk_def, SimpRHS] \\ gvs[]
-    \\ rw[Once OWHILE_THM, apply_def, apply_exc_def] )
+      rw[switch_BoolV_def, raise_def]
+      \\ rw[Once OWHILE_THM, stepk_def, apply_exc_def] )
+    \\ simp[switch_BoolV_def]
+    \\ IF_CASES_TAC \\ gvs[return_def]
+    >- (
+      rw[Once OWHILE_THM, stepk_def, apply_val_def]
+      \\ rw[Once OWHILE_THM, SimpRHS, stepk_def, apply_val_def]
+      \\ gvs[]
+      \\ rw[Once OWHILE_THM, stepk_def, apply_def] )
+    \\ reverse IF_CASES_TAC \\ gvs[raise_def]
+    >- (
+      qmatch_goalsub_rename_tac`ApplyVal v`
+      \\ rw[Once OWHILE_THM, stepk_def, apply_val_def, apply_exc_def]
+      \\ rw[Once OWHILE_THM, SimpRHS, stepk_def, apply_val_def] \\ gvs[]
+      \\ Cases_on`v` \\ gvs[apply_val_def, apply_exc_def]
+      \\ rw[Once OWHILE_THM, stepk_def, apply_val_def, apply_exc_def] )
+    \\ rw[bind_def]
+    \\ rw[Once OWHILE_THM, stepk_def, apply_val_def]
+    \\ first_x_assum drule \\ rw[cont_def]
+    \\ CASE_TAC
+    \\ reverse CASE_TAC \\ rw[Once OWHILE_THM, stepk_def, apply_val_def]
+    >- (
+      rw[Once OWHILE_THM, SimpRHS, stepk_def, apply_exc_def] \\ gvs[]
+      \\ qmatch_goalsub_rename_tac`apply_exc cx ex`
+      \\ Cases_on`ex` \\ gvs[apply_exc_def]
+      \\ rw[Once OWHILE_THM, stepk_def, apply_exc_def]  )
+    \\ rw[apply_tv_def, liftk1]
+    \\ CASE_TAC
+    \\ reverse CASE_TAC \\ rw[Once OWHILE_THM, stepk_def, apply_val_def]
+    >- (
+      rw[Once OWHILE_THM, SimpRHS, stepk_def, apply_exc_def] \\ gvs[]
+      \\ qmatch_goalsub_rename_tac`apply_exc cx ex`
+      \\ Cases_on`ex` \\ gvs[apply_exc_def]
+      \\ rw[Once OWHILE_THM, stepk_def, apply_exc_def]  )
+    \\ qmatch_goalsub_rename_tac`dest_StringV sv`
+    \\ Cases_on`sv` \\ gvs[dest_StringV_def, apply_val_def, lift_option_def,
+                           raise_def]
+    \\ TRY (
+      qmatch_asmsub_rename_tac`INL (StringV _ _)`
+      \\ rw[return_def]
+      \\ rw[Once OWHILE_THM, SimpRHS, stepk_def, apply_exc_def] \\ gvs[]
+      \\ rw[Once OWHILE_THM, apply_exc_def] \\ NO_TAC)
+    \\ rw[Once OWHILE_THM, SimpRHS, stepk_def, apply_exc_def] \\ gvs[]
+    \\ rw[Once OWHILE_THM, apply_exc_def])
   \\ conj_tac >- (
     rw[eval_stmt_cps_def, evaluate_def, bind_def]
     \\ CASE_TAC \\ rw[cont_def] \\ reverse CASE_TAC
